heap_lang/tests.v
@@ -1,6 +1,6 @@
 (** This file is essentially a bunch of testcases. *)
 Require Import program_logic.ownership.
-Require Import heap_lang.notation.
+Require Import heap_lang.notation heap_lang.substitution heap_lang.heap_lang_tactics.
 Import uPred.
 
 Module LangTests.
@@ -59,7 +59,8 @@ Module LiftingTests.
       let: "yp" := "y" + '1 in
       if "yp" < "x" then "pred" "x" "yp" else "y".
   Definition Pred : val :=
-    λ: "x", if "x" ≤ '0 then -FindPred (-"x" + '2) '0 else FindPred "x" '0.
+    λ: "x",
+      if "x" ≤ '0 then -FindPred (-"x" + '2) '0 else FindPred "x" '0.
 
   Lemma FindPred_spec n1 n2 E Q :
     (■ (n1 < n2) ∧ Q '(n2 - 1)) ⊑ wp E (FindPred 'n2 'n1)%L Q.
@@ -73,21 +74,21 @@ Module LiftingTests.
     rewrite ->(later_intro (Q _)).
     rewrite -!later_and; apply later_mono.
     (* Go on *)
-    rewrite -wp_let //= -later_intro.
-    rewrite -(wp_bindi (LetCtx _ _)) -wp_bin_op //= -wp_let //=.
-    rewrite -(wp_bindi (IfCtx _ _)) /= -!later_intro.
+    rewrite -wp_let' //= -later_intro.
+    rewrite -(wp_bindi (LetCtx _ _)) -wp_bin_op //= -wp_let' //= -!later_intro.
+    rewrite -(wp_bindi (IfCtx _ _)) /=.
     apply wp_lt=> ?.
-    - rewrite -wp_if_true.
-      rewrite -!later_intro (forall_elim (n1 + 1)) const_equiv; last omega.
+    - rewrite -wp_if_true -!later_intro.
+      rewrite (forall_elim (n1 + 1)) const_equiv; last omega.
       by rewrite left_id impl_elim_l.
     - assert (n1 = n2 - 1) as -> by omega.
-      rewrite -wp_if_false.
-      by rewrite -!later_intro -wp_value' // and_elim_r.
+      rewrite -wp_if_false -!later_intro.
+      by rewrite -wp_value' // and_elim_r.
   Qed.
 
   Lemma Pred_spec n E Q : ▷ Q (LitV (n - 1)) ⊑ wp E (Pred 'n)%L Q.
   Proof.
-    rewrite -wp_lam //=.
+    rewrite -wp_lam' //=.
     rewrite -(wp_bindi (IfCtx _ _)) /=.
     apply later_mono, wp_le=> Hn.
     - rewrite -wp_if_true.
@@ -99,8 +100,8 @@ Module LiftingTests.
       rewrite -FindPred_spec. apply and_intro; first by (apply const_intro; omega).
       rewrite -wp_un_op //= -later_intro.
       by assert (n - 1 = - (- n + 2 - 1)) as -> by omega.
-    - rewrite -wp_if_false.
-      rewrite -!later_intro -FindPred_spec.
+    - rewrite -wp_if_false -!later_intro.
+      rewrite -FindPred_spec.
       auto using and_intro, const_intro with omega.
   Qed.
 
@@ -108,7 +109,7 @@ Module LiftingTests.
     True ⊑ wp (Σ:=Σ) E (let: "x" := Pred '42 in Pred "x") (λ v, v = '40).
   Proof.
     intros E.
-    rewrite -(wp_bindi (LetCtx _ _)) -Pred_spec //= -wp_let //=.
+    rewrite -(wp_bindi (LetCtx _ _)) -Pred_spec //= -wp_let' //=.
     by rewrite -Pred_spec -!later_intro /=.
   Qed.
 End LiftingTests.
