heap_lang/substitution.v
@@ -1,0 +1,147 @@
+Require Export heap_lang.derived.
+
+(** We define an alternative notion of substitution [gsubst e x ev] that
+preserves the expression [e] syntactically in case the variable [x] does not
+occur freely in [e]. By syntactically, we mean that [e] is preserved without
+unfolding any Coq definitions. For example:
+
+<<
+  Definition id : val := λ: "x", "x".
+  Eval simpl in subst (id "y") "y" '10.   (* (Lam "x" "x") '10 *)
+  Eval simpl in gsubst (id "y") "y" '10.  (* id '10 *)
+>>
+
+For [gsubst e x ev] to work, [e] should not contain any opaque parts.
+
+The function [gsubst e x ev] differs in yet another way from [subst e x v].
+The function [gsubst] substitutes an expression [ev] whereas [subst]
+substitutes a value [v]. This way we avoid unnecessary conversion back and
+forth between values and expressions, which could also cause Coq definitions
+to be unfolded. For example, consider the rule [wp_rec'] from below:
+
+<<
+  Definition foo : val := rec: "f" "x" := ... .
+
+  Lemma wp_rec' E e1 f x erec e2 v Q :
+    e1 = Rec f x erec →
+    to_val e2 = Some v →
+    ▷ wp E (gsubst (gsubst erec f e1) x e2) Q ⊑ wp E (App e1 e2) Q.
+>>
+
+We ensure that [e1] is substituted instead of [RecV f x erec]. So, for example
+when taking [e1 := foo] we ensure that [foo] is substituted without being
+unfolded. *)
+
+(** * Implementation *)
+(** The core of [gsubst e x ev] is the partial function [gsubst_go e x ev] that
+returns [None] in case [x] does not occur freely in [e] and [Some e'] in case
+[x] occurs in [e]. The function [gsubst e x ev] is then simply defined as
+[from_option e (gsubst_go e x ev)]. *)
+Definition gsubst_lift {A B C} (f : A → B → C)
+    (x : A) (y : B) (mx : option A) (my : option B) : option C :=
+  match mx, my with
+  | Some x, Some y => Some (f x y)
+  | Some x, None => Some (f x y)
+  | None, Some y => Some (f x y)
+  | None, None => None
+  end.
+Fixpoint gsubst_go (e : expr) (x : string) (ev : expr) : option expr :=
+  match e with
+  | Var y => if decide (x = y ∧ x ≠ "") then Some ev else None
+  | Rec f y e =>
+     if decide (x ≠ f ∧ x ≠ y) then Rec f y <$> gsubst_go e x ev else None
+  | App e1 e2 => gsubst_lift App e1 e2 (gsubst_go e1 x ev) (gsubst_go e2 x ev)
+  | Lit l => None
+  | UnOp op e => UnOp op <$> gsubst_go e x ev
+  | BinOp op e1 e2 =>
+     gsubst_lift (BinOp op) e1 e2 (gsubst_go e1 x ev) (gsubst_go e2 x ev)
+  | If e0 e1 e2 =>
+     gsubst_lift id (If e0 e1) e2
+       (gsubst_lift If e0 e1 (gsubst_go e0 x ev) (gsubst_go e1 x ev))
+       (gsubst_go e2 x ev)
+  | Pair e1 e2 => gsubst_lift Pair e1 e2 (gsubst_go e1 x ev) (gsubst_go e2 x ev)
+  | Fst e => Fst <$> gsubst_go e x ev
+  | Snd e => Snd <$> gsubst_go e x ev
+  | InjL e => InjL <$> gsubst_go e x ev
+  | InjR e => InjR <$> gsubst_go e x ev
+  | Case e0 x1 e1 x2 e2 =>
+     gsubst_lift id (Case e0 x1 e1 x2) e2
+       (gsubst_lift (λ e0' e1', Case e0' x1 e1' x2) e0 e1
+         (gsubst_go e0 x ev)
+         (if decide (x ≠ x1) then gsubst_go e1 x ev else None))
+       (if decide (x ≠ x2) then gsubst_go e2 x ev else None)
+  | Fork e => Fork <$> gsubst_go e x ev
+  | Loc l => None
+  | Alloc e => Alloc <$> gsubst_go e x ev
+  | Load e => Load <$> gsubst_go e x ev
+  | Store e1 e2 => gsubst_lift Store e1 e2 (gsubst_go e1 x ev) (gsubst_go e2 x ev)
+  | Cas e0 e1 e2 =>
+     gsubst_lift id (Cas e0 e1) e2
+       (gsubst_lift Cas e0 e1 (gsubst_go e0 x ev) (gsubst_go e1 x ev))
+       (gsubst_go e2 x ev)
+  end.
+Definition gsubst (e : expr) (x : string) (ev : expr) : expr :=
+  from_option e (gsubst_go e x ev).
+
+(** * Simpl  *)
+(** Ensure that [simpl] unfolds [gsubst e x ev] when applied to a concrete term
+[e] and use [simpl nomatch] to ensure that it does not reduce in case [e]
+contains any opaque parts that block reduction. *)
+Arguments gsubst !_ _ _/ : simpl nomatch.
+
+(** We define heap_lang functions as values (see [id] above). In order to
+ensure too eager conversion to expressions, we block [simpl]. *)
+Arguments of_val : simpl never.
+
+(** * Correctness *)
+(** We prove that [gsubst] behaves like [subst] when substituting values. *)
+Lemma gsubst_None e x v : gsubst_go e x (of_val v) = None → e = subst e x v.
+Proof.
+  induction e; simpl; unfold gsubst_lift; intros;
+    repeat (simplify_option_equality || case_match); f_equal; auto.
+Qed.
+Lemma gsubst_correct e x v : gsubst e x (of_val v) = subst e x v.
+Proof.
+  unfold gsubst; destruct (gsubst_go e x (of_val v)) as [e'|] eqn:He; simpl;
+    last by apply gsubst_None.
+  revert e' He; induction e; simpl; unfold gsubst_lift; intros;
+    repeat (simplify_option_equality || case_match);
+    f_equal; auto using gsubst_None.
+Qed.
+
+(** * Weakest precondition rules *)
+Section wp.
+Context {Σ : iFunctor}.
+Implicit Types P : iProp heap_lang Σ.
+Implicit Types Q : val → iProp heap_lang Σ.
+Hint Resolve to_of_val.
+
+Lemma wp_rec' E e1 f x erec e2 v Q :
+  e1 = Rec f x erec →
+  to_val e2 = Some v →
+  ▷ wp E (gsubst (gsubst erec f e1) x e2) Q ⊑ wp E (App e1 e2) Q.
+Proof.
+  intros -> <-%of_to_val.
+  rewrite (gsubst_correct _ _ (RecV _ _ _)) gsubst_correct.
+  by apply wp_rec.
+Qed.
+
+Lemma wp_lam' E x ef e v Q :
+  to_val e = Some v → ▷ wp E (gsubst ef x e) Q ⊑ wp E (App (Lam x ef) e) Q.
+Proof. intros <-%of_to_val; rewrite gsubst_correct. by apply wp_lam. Qed.
+
+Lemma wp_let' E x e1 e2 v Q :
+  to_val e1 = Some v → ▷ wp E (gsubst e2 x e1) Q ⊑ wp E (Let x e1 e2) Q.
+Proof. apply wp_lam'. Qed.
+
+Lemma wp_case_inl' E e0 v0 x1 e1 x2 e2 Q :
+  to_val e0 = Some v0 →
+  ▷ wp E (gsubst e1 x1 e0) Q ⊑ wp E (Case (InjL e0) x1 e1 x2 e2) Q.
+Proof. intros <-%of_to_val; rewrite gsubst_correct. by apply wp_case_inl. Qed.
+
+Lemma wp_case_inr' E e0 v0 x1 e1 x2 e2 Q :
+  to_val e0 = Some v0 →
+  ▷ wp E (gsubst e2 x2 e0) Q ⊑ wp E (Case (InjR e0) x1 e1 x2 e2) Q.
+Proof. intros <-%of_to_val; rewrite gsubst_correct. by apply wp_case_inr. Qed.
+End wp.
+
